\section*{Група 1}
\begin{multline*}
{\mathbf 1.}\;
3 \log_{\sqrt{8}} 2 + 2^{-2\log_{\frac{1}{2}} 2} =
3\frac{\log_2 2}{\log_2 2^\frac{3}{2}} + 2^{-2 \log_{\frac{1}{2}} \left(\frac{1}{2}\right)^{-1}} =
3\frac{1}{\frac{3}{2}} + 2^{(-2)(-1)\log_{\frac{1}{2}} \frac{1}{2}} =\\
= \cancel{3}\frac{2}{\cancel{3}} + 2^2 = 2 + 4 = 6;
\end{multline*}

\begin{multline*}
{\mathbf 2.}\;
3\log_{\sqrt{64}} 4 + 4^{-2\log_{\frac{1}{4}} 3} =
3\frac{\log_4 4}{\log_4 4^{\frac{3}{2}}} + 4^{\frac{\log_4 \frac{1}{9}}{\log_4 \frac{1}{4}}} =
3\frac{1}{\frac{3}{2}} + 4^{\frac{-\log_4 9}{-\log_4 4}} =\\
= \cancel{3}\frac{2}{\cancel{3}} + 4^{\log_4 9} = 2 + 9 = 11;
\end{multline*}

\begin{multline*}
{\mathbf 9.}\;
\frac{\log_4 11 + \log_4 23}{\log_8 253} =
\frac{\log_4 11 + \log_4 23}{\log_8 (11 \cdot 23)} =
\frac{\log_4 11 + \log_4 23}{\log_8 11 + \log_8 23} =\\
= \frac{\log_4 11 + \log_4 23}{\frac{\log_4 11}{\log_4 8} + \frac{\log_4 23}{\log_4 8}} =
\cancel{\left(\log_4 11 + \log_4 23\right)} \cdot \frac{\log_4 8}{\cancel{\log_4 11 + \log_4 23}} =\\
= \frac{\log_2 2^3}{\log_2 2^2} = \frac{3}{2} = 1,5;
\end{multline*}

\begin{multline*}
{\mathbf 12.}\;
\log_4 a =
\left[a = \sin \frac{\pi}{6} = \sin 30^\circ = \frac{1}{2}\right] =
\log_4 \frac{1}{2} =
\frac{\log_2 2^{-1}}{\log_2 2^2} =\\
= -\frac{1}{2} = -0,5;
\end{multline*}

\begin{multline*}
{\mathbf 24.}\;
\frac{1}{\log_8 12} + \frac{1}{\log_{18} 12} =
\log_{12} 8 + \log_{12} 18 =
\log_{12} (8 \cdot 18) =
\log_{12} 144 = 2;
\end{multline*}

\begin{multline*}
{\mathbf 46.}\;
9^{\log_3 2} + 3^{1 - 2\log_3 2} =
3^{2\log_3 2} + 3^1 \cdot 3^{-2\log_3 2} =
3^{\log_3 4} + 3 \cdot 3^{\log_3 \frac{1}{4}} =\\
= 4 + \frac{3}{4} = 4,75;
\end{multline*}

\textbf{54.} $\log^2_3 \log_{\frac{1}{5}} \frac{1}{125} = \log^2_3 3 = \left(\log_3 3\right)^2 = 1$

\textbf{55.} $3^{\frac{3}{\log_7 3}} = 3^{\frac{3}{\frac{\log_3 3}{\log_3 7}}} = 3^{\frac{3}{\frac{1}{\log_3 7}}} = 3^{3\log_3 7} = 7^3 = 343;$
\section*{Група 2}

\begin{multline*}
{\mathbf 1.}\;
\log_3\log_2 \left(\sqrt[3]{2^k}\right)^{\frac{1}{3}} =
\log_3 \log_2 2^{\frac{k}{3} \cdot \frac{1}{3}} =
\log_3 \frac{k}{9} \log_2 2 =
\log_3 \frac{k}{9} =\\
= \log_3 k - \log_3 9 = 
\left[\log_3 k = 10\right] = 
10 - 2 = 8
\end{multline*}

\textbf{8.} $\left(\log_3 8\right)\left(\log_{17} 3\right)\left(\log_4 17\right) = \frac{\log_2 8}{\cancel{\log_2 3}} \cdot \frac{\cancel{\log_2 3}}{\cancel{\log_2 17}} \cdot \frac{\cancel{\log_2 17}}{\log_2 4} = \frac{3}{2} = 1,5;$

\begin{multline*}
{\mathbf 11.}\;
\left(2^{\log_4 \left(\sqrt{3} - 2\right)^2} + 3^{\log_3 \left(\sqrt{3} + 2\right)}\right)^2 =
\left(4^{\log_4 \left|\sqrt{3} - 2\right|} + 3^{\log_3 \left(\sqrt{3} + 2\right)}\right)^2 =\\
= \left(\;\left|\sqrt{3} - 2\right| + \sqrt{3} + 2\right)^2 =
\left(2 - \sqrt{3} + \sqrt{3} + 2\right)^2 = 16;
\end{multline*}

\begin{multline*}
{\mathbf 13.}\;
8 + \frac{1}{2}\log_{\frac{2}{3}} \left(6 - \sqrt{20}\right) + \frac{1}{2}\log_{\frac{2}{3}} \left(6 + \sqrt{20}\right) - \log_{\frac{2}{3}} 9 =\\
8 + \log_{\frac{2}{3}} \sqrt{6 - \sqrt{20}} + \log_{\frac{2}{3}} \sqrt{6 + \sqrt{20}} - \log_{\frac{2}{3}} 9 =\\
8 + \log_{\frac{2}{3}} \frac{\sqrt{\left(6 - \sqrt{20}\right)\left(6 + \sqrt{20}\right)}}{9} =
8 + \log_{\frac{2}{3}} \frac{\sqrt{36 - 20}}{9} =\\
8 + \log_{\frac{2}{3}} \frac{4}{9} = 8 + 2 = 10;
\end{multline*}

\begin{multline*}
{\mathbf 16.}\;
\frac{\log_2^2 14 \left(\log_2 14\right)\left(\log_2 7\right) - 2 \log_2^2 7}{\log_2 14 + 2\log_2 7} =\\
\frac{\left(\log_2 2 + \log_2 7\right)^2 + \left(\log_2 2 + \log_2 7\right)\left(\log_2 7\right) - 2\log_2^2 7}{\log_2 2 + \log_2 7 + 2\log_2 7} =\\
\frac{\left(1 + \log_2 7\right)^2 + \left(1 + \log_2 7\right)\left(\log_2 7\right) - 2\log_2^2 7}{1 + 3\log_2 7} =\\
\frac{1 + 2\log_2 7 + \cancel{\log_2^2 7} +\log_2 7 + \cancel{\log_2^2 7}- \cancel{2\log_2^2 7}}{1 + 3\log_2 7} =\\
= \frac{1 + 3\log_2 7}{1 + 3\log_2 7} = 1;
\end{multline*}
\section*{Група 3}

\begin{multline*}
{\mathbf 1.}\;
\log_{ab} x = \frac{1}{\log_x ab} = \frac{1}{\log_x a + \log_x b} = \frac{1}{\frac{1}{\log_a x} + \frac{1}{\log_b x}} =\\
= \left[\log_a x = 2, \log_b x = 3\right] = \frac{1}{\frac{1}{2} + \frac{1}{3}} = \frac{1}{\frac{5}{6}} = \frac{6}{5} = 1,2;
\end{multline*}

\begin{multline*}
{\mathbf 10.}\;
\left(\log_3 2 + \log_2 81 + 4\right)\left(\log_3 2 - 2\log_{18} 2\right)\log_2 3 - \log_3 2 =\\
= \left(\log_3 2 + \frac{\log_3 3^4}{\log_3 2} + 4\right)\left(\log_2 3 - \frac{2\log_3 2}{\log_3 (2 \cdot 3^2)}\right)\frac{1}{\log_3 2} - \log_3 2 =\\
= \frac{\log_3^2 2 + 4 + 4\log_3 2}{\log_3 2} \cdot \left(\log_3 2 - \frac{2\log_3 2}{\log_3 2 + 2}\right) \cdot \frac{1}{\log_3 2} - \log_3 2 =\\
= \frac{\left(\log_3 2 + 2\right)^{\cancel{2}}}{\cancel{\log_3 2}} \cdot \frac{\cancel{\log_3^2 2} + \cancel{2\log_3 2} - \cancel{2\log_3 2}}{\cancel{\log_3 2 + 2}} \cdot \frac{1}{\cancel{\log_3 2}} - \log_3 2 =\\
= \cancel{\log_3 2} + 2 - \cancel{\log_3 2} = 2;
\end{multline*}